chore: update automation

Arm/Memory/Separate.lean
@@ -177,10 +177,10 @@ Thus, it must be the case that (a + n).toNat = a.base.toNat + n
 -/
 theorem add_lt_of_mem_legal_of_lt
     (h : mem_legal a (a + n)) :
-    a.base.toNat + n.toNat < 2^64 := by
+    a.toNat + n.toNat < 2^64 := by
   simp only [mem_legal, decide_eq_true_eq,
     le_def, toNat_add, Nat.reducePow] at h
-  by_cases hadd : a.base.toNat + n.toNat < 2^64
+  by_cases hadd : a.toNat + n.toNat < 2^64
   · assumption
   · exfalso
     bv_omega
@@ -192,7 +192,7 @@ Thus, it must be the case that (a + n).toNat = a.base.toNat + n
 -/
 theorem toNat_add_distrib_of_mem_legal_of_lt
     (h : mem_legal a (a + n)) :
-    (a + n).toNat = a.base.toNat + n.toNat := by
+    (a + n).toNat = a.toNat + n.toNat := by
   simp only [add_def, toNat_ofNat, Nat.reducePow]
   rw [Nat.mod_eq_of_lt]
   apply add_lt_of_mem_legal_of_lt h
@@ -219,7 +219,7 @@ section NewDefinitions
 namespace Memory
 
 /-- A half open interval of memory [base..base+len). -/
-structure Buffer where
+structure Region where
   /-- Base pointer of the buffer. -/
   base : BitVec 64
   /-- Length of the buffer. -/
@@ -232,44 +232,44 @@ Thus `[buf..buf+buf.len)`is a valid range of memory.
 Note that the interval is left closed, right open, and thus `buf.len` is the
 number of bytes in the memory range.
 -/
-def Buffer.legal (b : Buffer) : Prop :=
+def Region.legal (b : Region) : Prop :=
   b.base.toNat + b.len ≤ 2^64
 
-/-- Build a `Buffer.legal` from a proof obligation that can be closed by `omega`. -/
-def Buffer.legal.of_omega {b : Buffer} (h : b.base.toNat + b.len ≤ 2^64) : b.legal := h
+/-- Build a `Region.legal` from a proof obligation that can be closed by `omega`. -/
+def Region.legal.of_omega {b : Region} (h : b.base.toNat + b.len ≤ 2^64) : b.legal := h
 
-theorem Buffer.legal.omega_def {b : Buffer} (h : b.legal) : b.base.toNat + b.len ≤ 2^64 := h
+theorem Region.legal.omega_def {b : Region} (h : b.legal) : b.base.toNat + b.len ≤ 2^64 := h
 
 /--
 @bollu: have proof automation exploit this.
-Equation lemma for `Buffer.legal`.
+Equation lemma for `Region.legal`.
 -/
-theorem Buffer.legal_def {b : Buffer}
+theorem Region.legal_def {b : Region}
   (h : b.legal) : b.base.toNat + b.len ≤ 2^64 := h
 
 /--
 The maximum size of the range we can choose to allocate is 2^64.
 @bollu: have proof automation exploit this.
 -/
-theorem Buffer.legal.size_le_two_pow {b : Buffer} (h : b.legal) : b.len ≤ 2 ^ 64 := by
-  rw [Buffer.legal] at h
+theorem Region.legal.size_le_two_pow {b : Region} (h : b.legal) : b.len ≤ 2 ^ 64 := by
+  rw [Region.legal] at h
   omega
 
 
 /--
 If we know that `[a..a+n)` is legal and `a'.toNat + n' < a.base.toNat + n`,
 then `[a'..a'+n')` is also legal. -/
-theorem Buffer.legal.of_Buffer.legal_of_lt
-    (h : Buffer.legal a) (hn : a'.base.toNat + a'.len ≤ a.base.toNat + a.len) :
-    Buffer.legal a' := by
-  unfold Buffer.legal at h ⊢
+theorem Region.legal.of_Region.legal_of_lt
+    (h : Region.legal a) (hn : a'.base.toNat + a'.len ≤ a.base.toNat + a.len) :
+    Region.legal a' := by
+  unfold Region.legal at h ⊢
   omega
 /--
 Legal in the new sense implies legal in the old sense.
 -/
-theorem mem_legal_of_Buffer.legal (h : Buffer.legal a) :
+theorem mem_legal_of_Region.legal (h : Region.legal a) :
     mem_legal a.base (a.base + (BitVec.ofNat 64 (a.len - 1))) := by
-  simp only [Buffer.legal, mem_legal, BitVec.le_def] at h ⊢
+  simp only [Region.legal, mem_legal, BitVec.le_def] at h ⊢
   rw [BitVec.toNat_add_eq_toNat_add_toNat]
   simp only [BitVec.toNat_ofNat, Nat.reducePow, Nat.le_add_right, decide_True]
   bv_omega
@@ -278,66 +278,66 @@ theorem mem_legal_of_Buffer.legal (h : Buffer.legal a) :
 Legal in the new sense implies legal in the old sense.
 Note that the subtraction could also have been written as `(b - a).toNat + 1`
 -/
-theorem Buffer.legal_of_mem_legal (h: mem_legal a b) : Buffer.legal { base := a , len := (b.toNat - a.toNat + 1) } := by
+theorem Region.legal_of_mem_legal (h: mem_legal a b) : Region.legal { base := a , len := (b.toNat - a.toNat + 1) } := by
   simp only [mem_legal, decide_eq_true_eq] at h
-  rw [Buffer.legal]
+  rw [Region.legal]
   bv_omega
 
-def Buffer.legal_of_Buffer.legal_of_lt (h : Buffer.legal a) (m : Nat) (hm : m ≤ a.len) :
-    Buffer.legal { a with len := m } := by
-  simp only [Buffer.legal, Nat.reducePow] at h ⊢
+def Region.legal_of_Region.legal_of_lt (h : Region.legal a) (m : Nat) (hm : m ≤ a.len) :
+    Region.legal { a with len := m } := by
+  simp only [Region.legal, Nat.reducePow] at h ⊢
   omega
 
 /--
-`mem_legal` is equivalent to `Buffer.legal`.
+`mem_legal` is equivalent to `Region.legal`.
 -/
-theorem mem_legal_iff_Buffer.legal : mem_legal a b ↔
-    Buffer.legal a ((b - a).toNat + 1) := by
+theorem mem_legal_iff_Region.legal : mem_legal a b ↔
+    Region.legal { base := a, len := ((b - a).toNat + 1) } := by
   constructor
   · intros h
     simp only [mem_legal, decide_eq_true_eq] at h
     rw [BitVec.toNat_sub_eq_toNat_sub_toNat_of_le h]
-    · simp only [Buffer.legal]
+    · simp only [Region.legal]
       omega
   · intros h
-    simp only [Buffer.legal] at h
+    simp only [Region.legal] at h
     simp only [mem_legal, BitVec.le_def, decide_eq_true_eq]
     bv_omega
 
 /--
-`Buffer.separate a an b bn` asserts that two memory regions [a..an) and [b..bn) are separate.
+`Region.separate a an b bn` asserts that two memory regions [a..an) and [b..bn) are separate.
 Note that we use *half open* intervals.
 In prose, we may notate this as `[a..an) ⟂ [b..bn)`.
 See also: Why numbering should start at zero (https://www.cs.utexas.edu/~EWD/ewd08xx/EWD831.PDF)
 -/
-structure Buffer.Separate (a b : Buffer) : Prop where
-  ha : Buffer.legal a
-  hb : Buffer.legal b
+structure Region.Separate (a b : Region) : Prop where
+  ha : Region.legal a
+  hb : Region.legal b
   h : a.base.toNat + a.len ≤ b.base.toNat ∨ a.base.toNat ≥ b.base.toNat + b.len
 
-scoped notation a " ⟂ " b  => (Buffer.Separate a b)
+scoped notation a " ⟂ " b  => (Region.Separate a b)
 
 
 /--
-Unfold the definition of `Subset` to write definitions that `omega` can process.
+Unfold the definition of `Region.Subset` to write definitions that `omega` can process.
 -/
-theorem Buffer.Separate.omega_def {a b : Buffer} (h : Buffer.Separate a b) :
+theorem Region.Separate.omega_def {a b : Region} (h : Region.Separate a b) :
   (a.base.toNat + a.len ≤ 2^64 ∧
   b.base.toNat + b.len ≤ 2^64 ∧
   (a.base.toNat + a.len ≤ b.base.toNat ∨ a.base.toNat ≥ b.base.toNat + b.len)) := by
   obtain ⟨ha, hb, hsplit⟩ := h
-  unfold Buffer.legal at ha hb
+  unfold Region.legal at ha hb
   omega
 
-/-- Build a Subset from a goal that `h` that can be closed by `omega`. -/
-theorem Buffer.Separate.of_omega {a b : Buffer}
+/-- Build a Region.Subset from a goal that `h` that can be closed by `omega`. -/
+theorem Region.Separate.of_omega {a b : Region}
     (h : a.base.toNat + a.len ≤ 2^64 ∧
     b.base.toNat + b.len ≤ 2^64 ∧
     (a.base.toNat + a.len ≤ b.base.toNat ∨ a.base.toNat ≥ b.base.toNat + b.len)) :
     a ⟂ b :=  by
   constructor
-  · unfold Buffer.legal; omega
-  · unfold Buffer.legal; omega
+  · unfold Region.legal; omega
+  · unfold Region.legal; omega
   · omega
 
 theorem BitVec.not_le_eq_lt {a b : BitVec w₁} : (¬ (a ≤ b)) ↔ b < a := by
@@ -346,18 +346,18 @@ theorem BitVec.not_le_eq_lt {a b : BitVec w₁} : (¬ (a ≤ b)) ↔ b < a := by
 
 /-#
 This is a theorem we ought to prove, which establishes the equivalence
-between the old and new defintions of 'Buffer.separate.
+between the old and new defintions of 'Region.separate.
 However, the proof is finicky, and so we leave it commented for now.
 -/
 /-
-theorem mem_separate_of_Buffer.separate (h : Buffer.separate a an b bn)
+theorem mem_separate_of_Region.separate (h : Region.separate a an b bn)
     (ha' : a' = a + (BitVec.ofNat w₁ (an - 1) ) (hb' : b' = b + (BitVec.ofNat w₁ (bn - 1)))
     (hlegala : mem_legal a an) (hlegalb: mem_legal b bn) :
     mem_separate a a' b b' := by
   simp [mem_separate]
   simp [mem_overlap]
   obtain ⟨ha, hb, hsep⟩ := h
-  simp [Buffer.legal] at ha hb
+  simp [Region.legal] at ha hb
   subst ha'
   subst hb'
   apply Classical.byContradiction
@@ -366,42 +366,42 @@ theorem mem_separate_of_Buffer.separate (h : Buffer.separate a an b bn)
   · sorry
 -/
 
-/-- `Subset a b` witnesses that `[a..a+an)` is a subset of `[b..b+bn)`.
+/-- `Region.Subset a b` witnesses that `[a..a+an)` is a subset of `[b..b+bn)`.
 In prose, we may notate this as `[a..an) ≤ [b..bn)`.
 -/
-structure Subset (a b : Buffer) : Prop where
+structure Region.Subset (a b : Region) : Prop where
   ha : a.legal
   hb : b.legal
   hstart : b.base.toNat ≤ a.base.toNat
   hend : a.base.toNat + a.len ≤ b.base.toNat + b.len
 
-scoped notation (name := subset) a " ⊆ " b  => (Subset a b)
+scoped notation (name := subset) a " ⊆ " b  => (Region.Subset a b)
 
 /--
-Unfold the definition of `Subset` to write definitions that `omega` can process.
+Unfold the definition of `Region.Subset` to write definitions that `omega` can process.
 -/
-theorem Subset.omega_def {a b : Buffer} (h : a ⊆ b) :
+theorem Region.Subset.omega_def {a b : Region} (h : a ⊆ b) :
   a.base.toNat + a.len ≤ 2^64 ∧
   b.base.toNat + b.len ≤ 2^64 ∧
   b.base.toNat ≤ a.base.toNat ∧
   a.base.toNat + a.len ≤ b.base.toNat + b.len := by
   obtain ⟨ha, hb, hstart, hend⟩ := h
-  unfold Buffer.legal at ha hb
+  unfold Region.legal at ha hb
   omega
 
-/-- Build a Subset from a goal that `h` that can be closed by `omega`. -/
-theorem Subset.of_omega {a b : Buffer}
+/-- Build a Region.Subset from a goal that `h` that can be closed by `omega`. -/
+theorem Region.Subset.of_omega {a b : Region}
   (h : a.base.toNat + a.len ≤ 2^64 ∧
   b.base.toNat + b.len ≤ 2^64 ∧
   b.base.toNat ≤ a.base.toNat ∧
-  a.base.toNat + a.len ≤ b.base + b.len) : Subset a b :=  by
+  a.base.toNat + a.len ≤ b.base.toNat + b.len) : Region.Subset a b :=  by
 constructor
-· unfold Buffer.legal; omega
-· unfold Buffer.legal; omega
+· unfold Region.legal; omega
+· unfold Region.legal; omega
 · omega
 · omega
 
-theorem Subset_refl {a : Buffer} (h : a.legal) : Subset a a where
+theorem Region.Subset_refl {a : Region} (h : a.legal) : Region.Subset a a where
   ha := h
   hb := h
   hstart := by simp only [BitVec.le_def, Nat.le_refl]
@@ -412,45 +412,44 @@ If `[a'..a'+an')` begins at least where `[a..an)` begins,
 and ends before `[a..an)` ends, and if `[a..an)` is a subset of `[b..bn)`,
 then `[a'..a'+an')` is a subset of `[b..bn)`.
 -/
-theorem Subset_of_le_of_le {a b a' : Buffer} (h : a ⊆ b)
+theorem Region.Subset_of_le_of_le {a b a' : Region} (h : a ⊆ b)
   (ha' : a.base.toNat ≤ a'.base.toNat) (han' : a'.base.toNat + a'.len ≤ a.base.toNat + a.len) :
-  Subset a' b where
+  Region.Subset a' b where
   ha := by
-    obtain ⟨ha, hb, hstart, hend⟩ := h
-    simp only [Buffer.legal, Nat.reducePow] at ha hb ⊢
+    obtain ⟨ha, hb, _, hend⟩ := h
+    simp only [Region.legal, Nat.reducePow] at ha hb ⊢
     omega
   hb := h.hb
   hstart := by
-    obtain ⟨ha, hb, hstart, hend⟩ := h
-    simp only [Buffer.legal, Nat.reducePow] at ha hb
+    obtain ⟨ha, hb, hstart, _⟩ := h
+    simp only [Region.legal, Nat.reducePow] at ha hb
     omega
   hend := by
-    obtain ⟨ha, hb, hstart, hend⟩ := h
-    simp only [Buffer.legal, Nat.reducePow] at ha hb
+    obtain ⟨ha, hb, _, hend⟩ := h
+    simp only [Region.legal, Nat.reducePow] at ha hb
     omega
 
 /-- if `[a..an) ≤ [b..bn)` and `[b..bn) ⟂ [c..cn)`,
 then `[a..an) ⟂ [c..cn)`.
-(Recall that `⟂` stands for `Buffer.separate`.)
+(Recall that `⟂` stands for `Region.separate`.)
 -/
-theorem Buffer.separate_of_Buffer.separate_of_Subset
-    (hsep : Separate b c)
-    (hsub : Subset a b) :
-    Subset a c := by
+theorem Region.separate_of_Region.separate_of_Region.Subset
+    (hsep : Region.Separate b c)
+    (hsub : Region.Subset a b) :
+    Separate a c := by
   obtain ⟨_, hsep₂, hsep₃⟩ := hsep
   obtain ⟨hsub₁, _, hsub₃, hsub₄⟩ := hsub
-  simp_all only [BitVec.le_def]
   constructor <;>
     solve
     | omega
     | assumption
 
--- `Subset` implies `mem_subset`.
-theorem mem_subset_of_Subset (h : Subset a b) (han : a.len > 0) (hbn : b.len > 0) :
+-- `Region.Subset` implies `mem_subset`.
+theorem mem_subset_of_Region.Subset (h : Region.Subset a b) (han : a.len > 0) (hbn : b.len > 0) :
   mem_subset a.base (a.base + BitVec.ofNat 64 (a.len - 1)) b.base (b.base + BitVec.ofNat 64 (b.len - 1)):= by
   unfold mem_subset
   obtain ⟨ha, hb, hstart, hend⟩ := h
-  unfold Buffer.legal at ha hb
+  unfold Region.legal at ha hb
   simp only [bitvec_rules, minimal_theory]
   by_cases hb : b.len = 2^64
   · left
@@ -458,7 +457,7 @@ theorem mem_subset_of_Subset (h : Subset a b) (han : a.len > 0) (hbn : b.len > 0
   · bv_omega
 
 /- value of read_mem_bytes when separate from the write. -/
-theorem read_bytes_write_bytes_eq_read_bytes_of_Buffer.separate {x y : Buffer}
+theorem read_bytes_write_bytes_eq_read_bytes_of_Region.separate {x y : Region}
     (hsep : x ⟂ y) -- separation
     (val : BitVec (y.len * 8)) :
     Memory.read_bytes x.len x.base (Memory.write_bytes y.len y.base val mem) =
@@ -476,7 +475,7 @@ theorem read_bytes_write_bytes_eq_read_bytes_of_Buffer.separate {x y : Buffer}
   bv_omega
 
 /- value of `read_mem_bytes'` when subset of the write. -/
-theorem read_bytes_write_bytes_eq_of_Subset
+theorem read_bytes_write_bytes_eq_of_Region.Subset
     (hsep : x ⊆ y) -- subset relation.
     (val : BitVec (y.len * 8)) :
     Memory.read_bytes x.len x.base (Memory.write_bytes y.len y.base val mem) =
@@ -486,7 +485,7 @@ theorem read_bytes_write_bytes_eq_of_Subset
   obtain ⟨hx, hy, hstart, hend⟩ := hsep
 
   obtain hx' := hx.size_le_two_pow
-  obtain hy' := Buffer.legal_def hy
+  obtain hy' := Region.legal_def hy
 
   rw [Memory.getLsb_read_bytes (by omega)]
   rw [Memory.getLsb_write_bytes (by omega)]
@@ -537,23 +536,25 @@ theorem read_bytes_write_bytes_eq_of_Subset
     · simp only [h₁, bitvec_rules, minimal_theory]
 
 /- value of read_mem_bytes when subset of another *read*. -/
-theorem read_bytes_eq_extractLsBytes_sub_of_Subset {a b : Buffer}
+theorem read_bytes_eq_extractLsBytes_sub_of_Region.Subset {a b : Region}
     {mem : Memory}
+    {val : BitVec (b.len * 8)}
     (hread : mem.read_bytes b.len b.base = val)
     (hsubset : a ⊆ b) :
-    mem.read_bytes an a = val.extractLsBytes (a.base.toNat - b.base.toNat) an := by
+    mem.read_bytes a.len a.base =
+      val.extractLsBytes (a.base.toNat - b.base.toNat) a.len := by
     have ⟨h1, h2, h3, h4⟩ := hsubset.omega_def
     apply BitVec.eq_of_extractLsByte_eq
     intros i
     rw [extractLsByte_read_bytes (by bv_omega)]
     rw [BitVec.extractLsByte_extractLsBytes]
-    by_cases h : i < an
+    by_cases h : i < a.len
     · simp only [h, ↓reduceIte]
       apply BitVec.eq_of_getLsb_eq
       intros j
       rw [← hread]
       rw [extractLsByte_read_bytes (by bv_omega)]
-      simp only [show a.base.toNat - b.base.toNat + i < bn by bv_omega, if_true]
+      simp only [show a.base.toNat - b.base.toNat + i < b.len by bv_omega, if_true]
       congr 2
       bv_omega
     · simp only [h, ↓reduceIte]
